Finish wf_types proof

pcuic/theories/PCUICWfUniverses.v
@@ -5,13 +5,23 @@ From MetaCoq.PCUIC Require Import PCUICAst PCUICInduction
      PCUICLiftSubst PCUICTyping PCUICWeakeningEnv PCUICWeakening PCUICInversion
      PCUICSubstitution PCUICReduction PCUICCumulativity PCUICGeneration
      PCUICUnivSubst PCUICParallelReductionConfluence PCUICWeakeningEnv
-     PCUICUnivSubstitution PCUICConversion.
+     PCUICUnivSubstitution PCUICConversion PCUICContexts.
 
 From Equations Require Import Equations.
 Require Import Equations.Prop.DepElim.
 Require Import ssreflect ssrbool.
 
 From MetaCoq.PCUIC Require Import PCUICInduction.
+
+Lemma forallbP {A} (P : A -> Prop) (p : A -> bool) l : (forall x, reflect (P x) (p x)) -> reflect (Forall P l) (forallb p l).
+Proof.
+  intros Hp.
+  apply: (iffP idP).
+  - induction l; rewrite /= //. move/andP => [pa pl].
+    constructor; auto. now apply/(Hp _).
+  - induction 1; rewrite /= // IHForall // andb_true_r.
+    now apply/(Hp _).
+Qed.
 
 Section CheckerFlags.
   Context {cf:checker_flags}.
@@ -54,10 +64,84 @@ Section CheckerFlags.
 
   Hint Resolve @wf_universe_type1 @wf_universe_super @wf_universe_sup @wf_universe_product : pcuic.
 
+
+  Definition wf_universeb_level Σ l := 
+    LevelSet.mem l (global_ext_levels Σ).
+
+  Definition wf_universe_level Σ l := 
+    LevelSet.In l (global_ext_levels Σ).
+    
+  Definition wf_universe_instance Σ u :=
+    Forall (wf_universe_level Σ) u.
+
+  Definition wf_universeb_instance Σ u :=
+    forallb (wf_universeb_level Σ) u.
+
+
+  Lemma wf_universe_levelP {Σ l} : reflect (wf_universe_level Σ l) (wf_universeb_level Σ l).
+  Proof.
+    unfold wf_universe_level, wf_universeb_level.
+    destruct LevelSet.mem eqn:ls; constructor.
+    now apply LevelSet.mem_spec in ls.
+    intros hin.
+    now apply LevelSet.mem_spec in hin.
+  Qed.
+
+  Lemma wf_universe_instanceP {Σ u} : reflect (wf_universe_instance Σ u) (wf_universeb_instance Σ u).
+  Proof.
+    unfold wf_universe_instance, wf_universeb_instance.
+    apply forallbP. intros x; apply wf_universe_levelP.
+  Qed.
+  
+  Lemma wf_universe_subst_instance (Σ : global_env_ext) univs u l :
+    wf Σ ->
+    wf_universe Σ l ->
+    wf_universe_instance (Σ.1, univs) u ->
+    sub_context_set (monomorphic_udecl Σ.2) (global_ext_context_set (Σ.1, univs)) ->
+    wf_universe (Σ.1, univs) (subst_instance u l). 
+  Proof.
+    destruct l; simpl; auto.
+    intros wfΣ Hl Hu sub e [[l n] [inl ->]]%In_subst_instance.
+    destruct l; simpl; auto.
+    - unfold global_ext_levels.
+      apply LS.union_spec. right.
+      apply global_levels_Set.
+    - specialize (Hl (Level.Level s, n) inl).
+      simpl in Hl.
+      destruct sub. unfold levels_of_udecl in H.
+      unfold global_ext_levels in Hl.
+      destruct Σ.2.
+      * eapply LS.union_spec in Hl.
+        destruct Hl as [Hl|Hl].
+        + now specialize (H _ Hl).
+        + eapply LS.union_spec. now right.
+      * eapply LS.union_spec in Hl as [Hl|Hl].
+        + simpl in Hl.
+          now apply monomorphic_level_notin_AUContext in Hl.
+        + apply LS.union_spec; now right.
+    - specialize (Hl (Level.Var n0, n) inl).
+      eapply LS.union_spec in Hl as [Hl|Hl].
+      + red in Hu.
+        unfold levels_of_udecl in Hl.
+        destruct Σ.2.
+        * simpl in Hu. simpl in *.
+          unfold subst_instance; simpl.
+          destruct nth_error eqn:hnth; simpl.
+          eapply nth_error_forall in Hu; eauto.
+          eapply LS.union_spec; right. eapply global_levels_Set.
+        * simpl in sub.
+          unfold subst_instance. simpl.
+          destruct (nth_error u n0) eqn:hnth.
+          2:{ simpl. rewrite hnth. eapply LS.union_spec; right; apply global_levels_Set. }
+          eapply nth_error_forall in Hu. 2:eauto. change (nth_error u n0) with (nth_error u n0) in *.
+          rewrite -> hnth. simpl. apply Hu.
+      + now apply not_var_global_levels in Hl.
+  Qed.
+
   Lemma wf_universe_instantiate Σ univs s u φ :
     wf Σ ->
     wf_universe (Σ, univs) s ->
-    consistent_instance_ext (Σ, φ) univs u ->
+    wf_universe_instance (Σ, φ) u ->
     sub_context_set (monomorphic_udecl univs) (global_ext_context_set (Σ, φ)) ->
     wf_universe (Σ, φ) (subst_instance_univ u s).
   Proof.
@@ -65,7 +149,133 @@ Section CheckerFlags.
     apply (wf_universe_subst_instance (Σ, univs) φ); auto.
   Qed.
 
-    Section WfUniverses.
+  Lemma subst_instance_instance_empty u : 
+    forallb (fun x => ~~ Level.is_var x) u ->
+    subst_instance_instance [] u = u.
+  Proof.
+    induction u; simpl; intros Hu; auto.
+    depelim Hu.
+    rewrite IHu //.
+    now destruct a => /= //; auto.
+    now destruct a => /= //; auto.
+  Qed.
+
+  Lemma wf_universe_level_mono Σ ctx u : 
+    wf Σ ->
+    on_udecl_prop Σ (Monomorphic_ctx ctx) ->
+    Forall (wf_universe_level (Σ, Monomorphic_ctx ctx)) u ->
+    forallb (fun x => ~~ Level.is_var x) u.
+  Proof.
+    intros wf uprop.
+    induction 1 => /= //.
+    destruct x eqn:isv => /= //.
+    apply LS.union_spec in H as [H|H]; simpl in H.
+    epose proof (@udecl_prop_in_var_poly _ (Σ, _) _ uprop H) as [ctx' eq].
+    discriminate.
+    now pose proof (not_var_global_levels _ wf _ H).
+  Qed.
+
+  Lemma wf_universe_level_sub Σ ctx univs u :
+    wf_universe_level (Σ, Monomorphic_ctx ctx) u ->
+    sub_context_set ctx (global_ext_context_set (Σ, univs)) ->
+    wf_universe_level (Σ, univs) u.
+  Proof.
+    intros wfx [sub _].
+    red in wfx |- *.
+    eapply LevelSet.union_spec in wfx; simpl in *.
+    destruct wfx as [wfx|wfx].
+    now specialize (sub _ wfx).
+    eapply LevelSet.union_spec. now right.
+  Qed.
+
+  Lemma wf_universe_instance_sub Σ ctx univs u :
+    wf_universe_instance (Σ, Monomorphic_ctx ctx) u ->
+    sub_context_set ctx (global_ext_context_set (Σ, univs)) ->
+    wf_universe_instance (Σ, univs) u.
+  Proof.
+    intros wfu [sub ?].
+    red in wfu |- *.
+    eapply Forall_impl; eauto.
+    intros; eapply wf_universe_level_sub; eauto.
+    red. split; auto.
+  Qed.
+
+  Lemma In_Level_global_ext_poly s Σ cst : 
+    LS.In (Level.Level s) (global_ext_levels (Σ, Polymorphic_ctx cst)) ->
+    LS.In (Level.Level s) (global_levels Σ).
+  Proof.
+    intros [hin|hin]%LS.union_spec.
+    simpl in hin.
+    now apply monomorphic_level_notin_AUContext in hin.
+    apply hin.
+  Qed.
+
+  Lemma Forall_In (A : Type) (P : A -> Prop) (l : list A) :
+    Forall P l -> (forall x : A, In x l -> P x).
+  Proof.
+    induction 1; simpl; auto.
+    intros x' [->|inx]; auto.
+  Qed.
+
+  Lemma wf_universe_instance_In {Σ u} : wf_universe_instance Σ u <-> 
+    (forall l, In l u -> LS.In l (global_ext_levels Σ)).
+  Proof.
+    unfold wf_universe_instance.
+    split; intros. eapply Forall_In in H; eauto.
+    apply In_Forall. auto.
+  Qed.
+
+  Lemma in_subst_instance_instance l u u' : 
+    In l (subst_instance_instance u u') ->
+    In l u \/ In l u' \/ l = Level.lSet.
+  Proof.
+    induction u'; simpl; auto.
+    intros [].
+    destruct a; simpl in *; subst; auto.
+    destruct (nth_in_or_default n u Level.lSet); auto.
+    specialize (IHu' H). intuition auto.
+  Qed.
+
+  Lemma wf_universe_subst_instance_instance Σ univs u u' φ : 
+    wf Σ ->
+    on_udecl_prop Σ univs ->
+    wf_universe_instance (Σ, univs) u' ->
+    wf_universe_instance (Σ, φ) u ->
+    sub_context_set (monomorphic_udecl univs) (global_ext_context_set (Σ, φ)) ->
+    wf_universe_instance (Σ, φ) (subst_instance_instance u u').
+  Proof.
+    intros wfΣ onup Hs cu subc.
+    destruct univs.
+    - red in Hs |- *.
+      unshelve epose proof (wf_universe_level_mono _ _ _ _ _ Hs); eauto.
+      eapply forallb_Forall in H. apply Forall_map.
+      solve_all. destruct x; simpl => //.
+      eapply LS.union_spec. right. eapply global_levels_Set.
+      eapply wf_universe_level_sub; eauto.
+    - simpl in subc.
+      clear subc onup.
+      red in Hs |- *.
+      eapply Forall_map, Forall_impl; eauto.
+      intros x wfx.
+      red in wfx. destruct x => /= //.
+      red.
+      eapply LS.union_spec; right.
+      eapply global_levels_Set.
+      eapply In_Level_global_ext_poly in wfx.
+      apply LS.union_spec; now right.
+      eapply in_var_global_ext in wfx; simpl in wfx; auto.
+      unfold AUContext.levels, AUContext.repr in wfx.
+      destruct cst as [? cst].
+      rewrite mapi_unfold in wfx.
+      eapply (proj1 (LevelSetProp.of_list_1 _ _)) in wfx.
+      apply SetoidList.InA_alt in wfx as [? [<- wfx]]. simpl in wfx.
+      eapply In_unfold in wfx.
+      destruct (nth_in_or_default n u (Level.lSet)).
+      red in cu. eapply Forall_In in cu; eauto. rewrite e.
+      red. eapply LS.union_spec. right. eapply global_levels_Set.
+  Qed.
+
+  Section WfUniverses.
     Context (Σ : global_env_ext).
 
     Definition wf_universeb (s : Universe.t) : bool :=
@@ -106,6 +316,7 @@ Section CheckerFlags.
       | tProj _ t => wf_universes t
       | tFix mfix _ | tCoFix mfix _ =>
         forallb (fun d => wf_universes d.(dtype) && wf_universes d.(dbody)) mfix
+      | tConst _ u | tInd _ u | tConstruct _ _ u => wf_universeb_instance Σ u
       | _ => true
       end.
 
@@ -170,12 +381,13 @@ Section CheckerFlags.
  
   Lemma wf_universes_inst {Σ : global_env_ext} univs t u : 
     wf Σ ->
+    on_udecl_prop Σ.1 univs ->
     sub_context_set (monomorphic_udecl univs) (global_ext_context_set Σ) ->
-    consistent_instance_ext Σ univs u ->
+    wf_universe_instance Σ u  ->
     wf_universes (Σ.1, univs) t ->
     wf_universes Σ (subst_instance u t).
   Proof.
-    intros wfΣ sub cu wft.
+    intros wfΣ onudecl sub cu wft.
     induction t using term_forall_list_ind; simpl in *; auto; try to_prop; 
       try apply /andP; to_wfu; intuition eauto 4.
 
@@ -183,6 +395,19 @@ Section CheckerFlags.
       eapply (wf_universe_subst_instance (Σ, univs)); auto.
 
     - apply /andP; to_wfu; intuition eauto 4.
+    - apply/wf_universe_instanceP.
+      eapply wf_universe_subst_instance_instance; eauto.
+      destruct Σ; simpl in *.
+      now move/wf_universe_instanceP: wft.
+    - apply/wf_universe_instanceP.
+      eapply wf_universe_subst_instance_instance; eauto.
+      destruct Σ; simpl in *.
+      now move/wf_universe_instanceP: wft.
+    - apply/wf_universe_instanceP.
+      eapply wf_universe_subst_instance_instance; eauto.
+      destruct Σ; simpl in *.
+      now move/wf_universe_instanceP: wft.
+    
     - apply /andP; to_wfu; intuition eauto 4.
     - rewrite forallb_map.
       red in X. solve_all.
@@ -208,6 +433,35 @@ Section CheckerFlags.
     eapply LS.union_spec. right; auto.
   Qed.
 
+  Lemma weaken_wf_universe_level Σ Σ' t : wf Σ' -> extends Σ.1 Σ' ->
+    wf_universe_level Σ t ->
+    wf_universe_level (Σ', Σ.2) t.
+  Proof.
+    intros wfΣ ext.
+    unfold wf_universe_level.
+    destruct t; simpl; auto;
+    intros; apply LS.union_spec.
+    - right. eapply global_levels_Set.
+    - eapply LS.union_spec in H as [H|H].
+      left; auto.
+      right; auto. simpl.
+      destruct ext. subst Σ'.
+      rewrite global_levels_ext.
+      eapply LS.union_spec. right; auto.
+    - eapply in_var_global_ext in H; eauto.
+      now eapply wf_extends.
+  Qed.
+
+  Lemma weaken_wf_universe_instance Σ Σ' t : wf Σ' -> extends Σ.1 Σ' ->
+    wf_universe_instance Σ t ->
+    wf_universe_instance (Σ', Σ.2) t.
+  Proof.
+    intros wfΣ ext.
+    unfold wf_universe_instance.
+    intros H; eapply Forall_impl; eauto.
+    intros. now eapply weaken_wf_universe_level.
+  Qed.
+
   Lemma weaken_wf_universes Σ Σ' t : wf Σ' -> extends Σ.1 Σ' ->
     wf_universes Σ t ->
     wf_universes (Σ', Σ.2) t.
@@ -218,6 +472,12 @@ Section CheckerFlags.
 
   - now eapply weaken_wf_universe.
   - apply /andP; to_wfu; intuition eauto 4.
+  - apply /wf_universe_instanceP; apply weaken_wf_universe_instance; eauto.
+    now apply /wf_universe_instanceP.
+  - apply /wf_universe_instanceP; apply weaken_wf_universe_instance; eauto.
+    now apply /wf_universe_instanceP.
+  - apply /wf_universe_instanceP; apply weaken_wf_universe_instance; eauto.
+    now apply /wf_universe_instanceP.
   - apply /andP; to_wfu; intuition eauto 4.
   - red in X; solve_all.
   - red in X. solve_all. to_prop.
@@ -229,13 +489,14 @@ Section CheckerFlags.
   Lemma wf_universes_weaken_full : weaken_env_prop_full (fun Σ Γ t T => 
       wf_universes Σ t && wf_universes Σ T).
   Proof.
-    red. intros.
+    red. intros.     
     to_prop; apply /andP; split; now apply weaken_wf_universes.
   Qed.
 
   Lemma wf_universes_weaken :
     weaken_env_prop
-      (lift_typing (fun Σ Γ (t T : term) => wf_universes Σ t && wf_universes Σ T)).
+      (lift_typing (fun Σ Γ (t T : term) =>
+        wf_universes Σ t && wf_universes Σ T)).
   Proof.
     red. intros.
     unfold lift_typing in *. destruct T. now eapply (wf_universes_weaken_full (_, _)).
@@ -243,11 +504,15 @@ Section CheckerFlags.
   Qed.
 
   Lemma wf_universes_inds Σ mind u bodies : 
+    wf_universe_instance Σ u ->
     All (fun t : term => wf_universes Σ t) (inds mind u bodies).
   Proof.
+    intros wfu.
     unfold inds.
     generalize #|bodies|.
     induction n; simpl; auto.
+    constructor; auto.
+    simpl. now apply /wf_universe_instanceP.
   Qed.
 
   Lemma wf_universes_mkApps Σ f args : 
@@ -274,68 +539,213 @@ Section CheckerFlags.
     apply IHΔ. apply X.
   Qed.
 
+  Lemma consistent_instance_ext_wf Σ univs u : consistent_instance_ext Σ univs u ->
+    wf_universe_instance Σ u.
+  Proof.
+    destruct univs; simpl.
+    - destruct u => // /=.
+      intros _. constructor.
+    - intros [H%forallb_Forall [H' H'']].
+      eapply Forall_impl; eauto.
+      simpl; intros. now eapply LS.mem_spec in H0.
+  Qed.
 
+  Ltac specIH :=
+    repeat match goal with
+    | [ H : on_udecl _ _, H' : on_udecl _ _ -> _ |- _ ] => specialize (H' H)
+    end.
+
+  Local Lemma wf_type_local_ctx_smash (Σ : global_env_ext) mdecl args sort :
+    type_local_ctx
+    (lift_typing
+       (fun (Σ : PCUICEnvironment.global_env_ext)
+          (_ : PCUICEnvironment.context) (t T : term) =>
+        wf_universes Σ t && wf_universes Σ T)) (Σ.1, ind_universes mdecl)
+    (arities_context (ind_bodies mdecl),,, ind_params mdecl)
+    args sort ->
+    type_local_ctx
+    (lift_typing
+       (fun (Σ : PCUICEnvironment.global_env_ext)
+          (_ : PCUICEnvironment.context) (t T : term) =>
+        wf_universes Σ t && wf_universes Σ T)) (Σ.1, ind_universes mdecl)
+    (arities_context (ind_bodies mdecl),,, ind_params mdecl)
+    (smash_context [] args) sort.
+  Proof.
+    induction args as [|[na [b|] ty] args]; simpl; auto.
+    intros [].
+    rewrite subst_context_nil. auto.
+    intros [].
+    rewrite smash_context_acc /=. split. auto.
+    rewrite wf_universes_subst.
+    clear -t. generalize 0.
+    induction args as [|[na [b|] ty] args]; simpl in *; auto.
+    destruct t as [? [[s wf] [? ?]%MCProd.andP]].
+    constructor; auto.
+    rewrite wf_universes_subst. apply IHargs; auto.
+    now rewrite wf_universes_lift.
+    constructor => //. now apply IHargs.
+    now rewrite wf_universes_lift.
+  Qed.
+
+  Lemma wf_type_local_ctx_nth_error Σ P Γ Δ s n d : 
+    type_local_ctx P Σ Γ Δ s -> 
+    nth_error Δ n = Some d ->
+    ∑ Γ' t, P Σ Γ' (decl_type d) t.
+  Proof.
+    induction Δ as [|[na [b|] ty] Δ] in n |- *; simpl; auto.
+    - now rewrite nth_error_nil.
+    - intros [h [h' h'']].
+      destruct n. simpl. move=> [= <-] /=. do 2 eexists; eauto.
+      now simpl; apply IHΔ.
+    - intros [h h'].
+      destruct n. simpl. move=> [= <-] /=. eexists; eauto.
+      now simpl; apply IHΔ.
+  Qed.
+
+  Lemma In_unfold_var x n : In x (unfold n Level.Var) <-> exists k, k < n /\ (x = Level.Var k).
+  Proof.
+    split.
+    - induction n => /= //.
+      intros [hin|hin]%in_app_or.
+      destruct (IHn hin) as [k [lt eq]].
+      exists k; auto.
+      destruct hin => //. subst x.
+      eexists; eauto.
+    - intros [k [lt ->]].
+      induction n in k, lt |- *. lia.
+      simpl. apply in_or_app.
+      destruct (lt_dec k n). left; auto.
+      right. left. f_equal. lia.      
+  Qed.
+
+  Lemma wf_abstract_instance Σ decl :
+    wf_universe_instance (Σ, decl) (PCUICLookup.abstract_instance decl).
+  Proof.
+    destruct decl as [|[u cst]]=> /= //.
+    red. constructor.
+    rewrite /UContext.instance /AUContext.repr /=.
+    rewrite mapi_unfold.
+    red. eapply In_Forall.
+    intros x hin. eapply In_unfold_var in hin as [k [lt eq]].
+    subst x. red.
+    eapply LS.union_spec; left. simpl.
+    rewrite /AUContext.levels /= mapi_unfold.
+    eapply (proj2 (LevelSetProp.of_list_1 _ _)).
+    apply SetoidList.InA_alt. eexists; split; eauto.
+    eapply In_unfold_var. exists k; split; eauto.
+  Qed.
+
+  Definition wf_decl_universes Σ d :=
+    option_default (wf_universes Σ) d.(decl_body) true &&
+    wf_universes Σ d.(decl_type).
+  
+  Definition wf_ctx_universes Σ Γ :=
+    forallb (wf_decl_universes Σ) Γ.
+  
+  Lemma wf_universes_it_mkProd_or_LetIn {Σ Γ T} : 
+    wf_universes Σ (it_mkProd_or_LetIn Γ T) = wf_ctx_universes Σ Γ && wf_universes Σ T.
+  Proof.
+    induction Γ as [ |[na [b|] ty] Γ] using rev_ind; simpl; auto;
+      now rewrite it_mkProd_or_LetIn_app /= IHΓ /wf_ctx_universes forallb_app /=
+      {3}/wf_decl_universes; cbn; bool_congr.
+  Qed.
+  
+  Lemma wf_projs Σ ind npars p :
+    All (fun t : term => wf_universes Σ t) (projs ind npars p).
+  Proof.
+    induction p; simpl; auto.
+  Qed.
+
+  Lemma wf_extended_subst Σ Γ n :
+    wf_ctx_universes Σ Γ ->
+    All (fun t : term => wf_universes Σ t) (extended_subst Γ n).
+  Proof.
+    induction Γ as [|[na [b|] ty] Γ] in n |- *; simpl; auto.
+    move=> /andP []; rewrite /wf_decl_universes /= => /andP [] wfb wfty wfΓ.
+    constructor; eauto. rewrite wf_universes_subst //. now apply IHΓ.
+    now rewrite wf_universes_lift. eauto.
+    move=> /andP []; rewrite /wf_decl_universes /= => wfty wfΓ.
+    constructor; eauto.
+  Qed.
 
   Theorem wf_types :
-    env_prop (fun Σ Γ t T => wf_universes Σ t && wf_universes Σ T)
+    env_prop (fun Σ Γ t T => 
+      wf_universes Σ t && wf_universes Σ T)
       (fun Σ Γ wfΓ =>
       All_local_env_over typing
       (fun (Σ : global_env_ext) (Γ : context) (_ : wf_local Σ Γ) 
          (t T : term) (_ : Σ;;; Γ |- t : T) => wf_universes Σ t && wf_universes Σ T) Σ Γ
       wfΓ).
   Proof.
-    apply typing_ind_env; intros; rename_all_hyps; simpl; to_prop; simpl; auto.
+    apply typing_ind_env; intros; rename_all_hyps; simpl; specIH; to_prop; simpl; auto.
 
     - rewrite wf_universes_lift.
       destruct (nth_error_All_local_env_over heq_nth_error X) as [HΓ' Hd].
       destruct decl as [na [b|] ty]; cbn -[skipn] in *.
-      + now destruct Hd as [Hd _]; to_prop.
+      + destruct Hd as [Hd _]; now to_prop.
       + destruct lookup_wf_local_decl; cbn -[skipn] in *.
         destruct o. now simpl in Hd; to_prop.
 
     - apply/andP; split; to_wfu; eauto with pcuic.
        
-    - simpl in *; to_wfu. eauto with pcuic.
+    - simpl in *; to_wfu; eauto with pcuic.
     - rewrite wf_universes_subst. constructor. to_wfu; auto. constructor.
       now move/andP: H3 => [].
 
-    - pose proof (declared_constant_inv _ _ _ _ wf_universes_weaken wf X H).
+    - apply/andP; split.
+      { apply/wf_universe_instanceP.
+        eapply consistent_instance_ext_wf; eauto. }
+      pose proof (declared_constant_inv _ _ _ _ wf_universes_weaken wf X H).
       red in X1; cbn in X1.
       destruct (cst_body decl).
       * to_prop.
-        eapply wf_universes_inst; eauto.
         epose proof (weaken_lookup_on_global_env'' Σ.1 _ _ wf H).
+        epose proof (weaken_lookup_on_global_env' Σ.1 _ _ wf H).
+        eapply wf_universes_inst. 2:eauto. all:eauto.
         simpl in H3.
         eapply sub_context_set_trans; eauto.
         eapply global_context_set_sub_ext.
+        now eapply consistent_instance_ext_wf.
       * move: X1 => [s /andP[Hc _]].
         to_prop.
         eapply wf_universes_inst; eauto.
+        exact (weaken_lookup_on_global_env' Σ.1 _ _ wf H).
         epose proof (weaken_lookup_on_global_env'' Σ.1 _ _ wf H).
-        simpl in H1.
         eapply sub_context_set_trans; eauto.
         eapply global_context_set_sub_ext.
+        now eapply consistent_instance_ext_wf.
 
-    - pose proof (declared_inductive_inv wf_universes_weaken wf X isdecl).
+    - apply/andP; split.
+      { apply/wf_universe_instanceP.
+        eapply consistent_instance_ext_wf; eauto. }
+      pose proof (declared_inductive_inv wf_universes_weaken wf X isdecl).
       cbn in X1. eapply onArity in X1. cbn in X1.
-      move: X1 => [s /andP[Hind _]].
+      move: X1 => [s /andP[Hind ?]].
       eapply wf_universes_inst; eauto.
+      exact (weaken_lookup_on_global_env' Σ.1 _ _ wf (proj1 isdecl)).
       generalize (weaken_lookup_on_global_env'' Σ.1 _ _ wf (proj1 isdecl)).
       simpl. intros H'.
       eapply sub_context_set_trans; eauto.
       eapply global_context_set_sub_ext.
+      now eapply consistent_instance_ext_wf.
 
-    - pose proof (declared_constructor_inv wf_universes_weaken wf X isdecl) as [sc [nthe onc]].
+    - apply/andP; split.
+      { apply/wf_universe_instanceP.
+        eapply consistent_instance_ext_wf; eauto. }
+      pose proof (declared_constructor_inv wf_universes_weaken wf X isdecl) as [sc [nthe onc]].
       unfold type_of_constructor.
       rewrite wf_universes_subst.
-      apply wf_universes_inds.
+      { apply wf_universes_inds.
+        now eapply consistent_instance_ext_wf. }
       eapply on_ctype in onc. cbn in onc.
       move: onc=> [_ /andP[onc _]].
       eapply wf_universes_inst; eauto.
+      exact (weaken_lookup_on_global_env' Σ.1 _ _ wf (proj1 (proj1 isdecl))).
       generalize (weaken_lookup_on_global_env'' Σ.1 _ _ wf (proj1 (proj1 isdecl))).
       simpl. intros H'.
       eapply sub_context_set_trans; eauto.
       eapply global_context_set_sub_ext.
+      now eapply consistent_instance_ext_wf.
     
     - apply /andP. split.
       solve_all. cbn in *. now to_prop.
@@ -354,11 +764,44 @@ Section CheckerFlags.
       destruct (declared_inductive_inv); simpl in *.
       destruct ind_cshapes as [|cs []] => //.
       destruct X1. red in o. subst ty.
-      destruct nth_error eqn:heq.
+      destruct nth_error eqn:heq => //.
       destruct o as [_ ->].
-      assert (wf_universes (Σ.1, ind_universes mdecl) (decl_type c0)).
-      destruct p0 as [[tyctx _] _].
-      all:admit.
+      rewrite wf_universes_mkApps in H1.
+      move/andP: H1 => [/wf_universe_instanceP wfu wfargs].
+
+      eapply (wf_universes_inst (ind_universes mdecl)); eauto.
+      exact (weaken_lookup_on_global_env' Σ.1 _ _ wf (proj1 (proj1 isdecl))).
+      generalize (weaken_lookup_on_global_env'' Σ.1 _ _ wf (proj1 (proj1 isdecl))).
+      simpl. intros H'.
+      eapply sub_context_set_trans; eauto.
+      eapply global_context_set_sub_ext.
+      rewrite wf_universes_subst.
+      eapply wf_universes_inds; eauto.
+      eapply wf_abstract_instance.
+      rewrite wf_universes_subst. apply wf_projs.
+      rewrite wf_universes_lift.
+      destruct p0 as [[? ?] ?].
+      rewrite smash_context_app smash_context_acc in heq.
+      autorewrite with len in heq. rewrite nth_error_app_lt in heq.
+      autorewrite with len. lia.
+      rewrite nth_error_subst_context in heq.
+      autorewrite with len in heq. simpl in heq.
+      epose proof (nth_error_lift_context_eq _ (smash_context [] (ind_params mdecl)) _ _).
+      autorewrite with len in H. simpl in H. rewrite -> H in heq. clear H.
+      autorewrite with len in heq.
+      simpl in heq.
+      destruct nth_error eqn:hnth; simpl in * => //.
+      noconf heq. simpl.
+      rewrite wf_universes_subst.
+      apply wf_extended_subst.
+      rewrite ind_arity_eq in onArity. destruct onArity as [s Hs].
+      rewrite wf_universes_it_mkProd_or_LetIn in Hs.
+      now move/andP: Hs => /andP /andP [] /andP [].
+      rewrite wf_universes_lift.
+      eapply wf_type_local_ctx_smash in t.
+      eapply wf_type_local_ctx_nth_error in t as [? [? H]]; eauto.
+      red in H. destruct x0. now move/andP: H => [].
+      now destruct H as [s [Hs _]%MCProd.andP].
     
     - apply/andP; split; auto.
       solve_all. move:a => [s [Hty /andP[wfty wfs]]].
@@ -371,7 +814,7 @@ Section CheckerFlags.
       to_prop. now rewrite wfty.
       eapply nth_error_all in X0; eauto.
       simpl in X0. now move: X0 => [s [Hty /andP[wfty _]]].
-  Admitted.
+  Qed.
 
   Lemma typing_wf_universes {Σ : global_env_ext} {Γ t T} : 
     wf Σ ->
@@ -393,21 +836,6 @@ Section CheckerFlags.
   Lemma isType_wf_universes {Σ Γ T} : wf Σ.1 -> isType Σ Γ T -> wf_universes Σ T.
   Proof.
     intros wfΣ [s Hs]. now eapply typing_wf_universes in Hs as [HT _]%MCProd.andP.
-  Qed.
-  
-  Definition wf_decl_universes Σ d :=
-    option_default (wf_universes Σ) d.(decl_body) true &&
-    wf_universes Σ d.(decl_type).
-  
-  Definition wf_ctx_universes Σ Γ :=
-    forallb (wf_decl_universes Σ) Γ.
-  
-  Lemma wf_universes_it_mkProd_or_LetIn {Σ Γ T} : 
-    wf_universes Σ (it_mkProd_or_LetIn Γ T) = wf_ctx_universes Σ Γ && wf_universes Σ T.
-  Proof.
-    induction Γ as [ |[na [b|] ty] Γ] using rev_ind; simpl; auto;
-      now rewrite it_mkProd_or_LetIn_app /= IHΓ /wf_ctx_universes forallb_app /=
-      {3}/wf_decl_universes; cbn; bool_congr.
   Qed.
   
 End CheckerFlags.
